src/ocaml/gen_our.ml
@@ -1,0 +1,1 @@
+../generated/gen_our.ml
