src/Export_code.thy
@@ -1,9 +1,12 @@
 theory Export_code
 imports Find_tree_stack Insert_tree_stack Delete_tree_stack "~~/src/HOL/Library/Code_Target_Numeral"
+"~~/src/HOL/Library/Code_Char"
 begin
 
 
 export_code "Code_Numeral.nat_of_integer" "Code_Numeral.int_of_integer" 
+
+key_ord
 
 dest_core
 
@@ -16,6 +19,10 @@ mk_its_state step_its dest_its_state
 mk_dts_state step_dts
   wellformed_dts_state wf_dts_trans Delete_tree_stack.focus_to_leaves
 
-in OCaml file "ocaml/btree_generated.ml"
+in OCaml file "generated/gen_btree.ml"
+
+print_codesetup
+
+print_codeproc
 
 end
