src/Key_value_types.thy
@@ -1,0 +1,32 @@
+theory Key_value_types
+imports Prelude
+begin
+
+(* we separate the types to make it easier to functorize the generated ocaml *)
+
+(* this makes code export easier; of course, key is abstract *)
+datatype key = Private_key nat
+
+(* FIXME really an abstract parameter; this for code export *)
+definition key_ord :: "key => key => int"  where (* as ocaml compare *)
+"key_ord k1 k2 = failwith ''key_ord''"
+
+datatype value_t = Private_value nat
+
+(*
+(* nonsense to get code export to work *)
+instantiation key :: equal begin
+definition equal_key :: "key \<Rightarrow> key \<Rightarrow> bool" where "equal_key = (op = )" 
+instance by intro_classes (simp add: equal_key_def)
+end
+*)
+
+
+
+
+type_synonym kv_t = "key * value_t"
+type_synonym kvs_t = "kv_t list"
+
+
+
+end
