src/ocaml/bash_env.sh
@@ -1,0 +1,23 @@
+set -a # export all vars
+# set -x # debug
+
+root=$(realpath $(dirname $BASH_SOURCE))/../..
+
+ # if using nix, this may not be present
+test -f $root/config.sh && source $root/config.sh
+
+PKGS=""
+SYNTAX="" # "-syntax camlp4o" # simplify: use for every file
+
+# 8~"pattern-matching is not exhaustive"; 
+# 11~"this match case is unused";
+# 26~"unused variable s2"
+WARN="-w @f@p@u@s@40-8-11-26"
+
+# these include syntax, so should work on all files; may be overridden in ocamlc.sh
+  ocamlc="$DISABLE_BYTE ocamlfind ocamlc   $WARN nums.cma $PKGS $SYNTAX"
+ocamlopt="$DISABLE_NTVE ocamlfind ocamlopt $WARN nums.cmxa $PKGS $SYNTAX"
+ocamldep="ocamlfind ocamldep $PKGS"
+
+mk_cma="$DISABLE_BYTE ocamlfind ocamlc"
+mk_cmxa="$DISABLE_NTVE ocamlfind ocamlopt"
